vvequiv/NetlistSemantics.v
@@ -1,6 +1,9 @@
 From Coq Require Import BinNums.
 From Coq Require Import BinNat.
 From Coq Require Import BinPos.
+From Coq Require Import List.
+From Coq Require FMaps.
+From Coq Require FMapFacts.
 
 From vvequiv Require Import Netlist.
 From vvequiv Require Import Common.
@@ -8,56 +11,176 @@ From vvequiv Require Import Bitvector.
 
 From Equations Require Import Equations.
 
-Import Bitvector (bv, mkBV).
+Import Bitvector.
 Import Netlist.
 
 (** Based on Lööw (2021) Lutsig: a verified Verilog compiler for verified circuit development, ACM. *)
 
 Definition RandomSource := nat -> bool.
 
-Definition ExternalState := NameMap.t bv.
+Equations input_port_in_map : NameMap.t bv -> (name * port_direction) -> Prop :=
+| map, (n, PortIn) => NameMap.In n map
+| map, (n, PortOut) => True.
 
-Definition RegisterState := NameMap.t bv.
+Record ExternalState (c : circuit) :=
+  MkExternalState
+    { external_state_map :> NameMap.t bv
+    ; external_state_wf : Forall (input_port_in_map external_state_map) (circuitPorts c)
+    }.
 
-Definition VariableState := NameMap.t bv.
+Arguments MkExternalState [_] _ _.
 
-Record CircuitState :=
+Equations register_in_map : NameMap.t bv -> register_declaration -> Prop :=
+| map, MkRegister _ n _ _ => NameMap.In n map.
+
+Record RegisterState (c : circuit) :=
+  MkRegisterState
+    { register_state_map :> NameMap.t bv
+    ; register_state_wf : Forall (register_in_map register_state_map) (circuitRegisters c)
+    }.
+
+Arguments MkRegisterState [_] _ _.
+
+Equations variable_in_map : NameMap.t bv -> variable -> Prop :=
+| map, Var _ n => NameMap.In n map.
+
+Record VariableState (c : circuit) :=
+  MkVariableState
+    { variable_state_map :> NameMap.t bv
+    ; variable_state_wf : Forall (variable_in_map variable_state_map) (circuitVariables c)
+    }.
+
+Arguments MkVariableState [_] _ _.
+
+Record CircuitState (c : circuit) :=
   MkCircuitState
-    { external : ExternalState
-    ; registers : RegisterState
-    ; variables : VariableState
+    { external : ExternalState c
+    ; registers : RegisterState c
+    ; variables : VariableState c
     }
 .
+
+Arguments MkCircuitState [_].
+Arguments external [_] _.
+Arguments registers [_] _.
+Arguments variables [_] _.
 
 Set Primitive Projections.
 
 Equations varWidth : variable -> positive :=
   varWidth (Var (Logic w) _) := w.
 
-Equations input_run : CircuitState -> input -> bv :=
-  input_run st (InConstant c) := c;
-  input_run st (InVar v) :=
-    (* TODO: Statically guarantee that this lookup can't fail so that we can
-    avoid returning a meaningless zero *)
-    opt_or_else
-      (opt_or
-         (NameMap.find v.(varName) st.(registers))
-         (NameMap.find v.(varName) st.(variables)))
-      (mkBV 0%N (varWidth v)).
+Equations var_reg_match : variable -> register_declaration -> Prop :=
+| Var var_type var_name, MkRegister reg_type reg_name _ _ =>
+    var_type = reg_type /\ var_name = reg_name.
 
-Equations cell_run : CircuitState -> cell -> CircuitState :=
-  cell_run st (Add (OutVar (Var _ out)) in1 in2) :=
-    let val1 := input_run st in1 in
-    let val2 := input_run st in2 in
-    (* let result := bv_add val1 val2 in *)
-    let result := (mkBV 0%N 32%positive) in
+Equations input_in_circuit : circuit -> input -> Prop :=
+| _, InConstant _ => True
+| c, InVar v => In v (circuitVariables c) \/ Exists (var_reg_match v) (circuitRegisters c).
+
+Equations output_in_circuit : circuit -> output -> Prop :=
+| c, OutVar v => In v (circuitVariables c) \/ Exists (var_reg_match v) (circuitRegisters c).
+
+Equations cell_in_circuit : circuit -> cell -> Prop :=
+| c, Add out in1 in2 _ _ =>
+    output_in_circuit c out
+    /\ input_in_circuit c in1
+    /\ input_in_circuit c in2
+| c, Subtract out in1 in2 _ _ =>
+    output_in_circuit c out
+    /\ input_in_circuit c in1
+    /\ input_in_circuit c in2
+| c, Id out in1 _ =>
+    output_in_circuit c out
+    /\ input_in_circuit c in1
+| c, Convert out in1 =>
+    output_in_circuit c out
+    /\ input_in_circuit c in1
+.
+
+Equations input_run {c} (st : CircuitState c) (i : input) (input_wf : input_in_circuit c i) : bv :=
+  input_run st (InConstant const) _ := const;
+  input_run st (InVar v) input_wf := _. (* TODO: Do this pattern match in gallina instead of tactics *)
+Next Obligation.
+  destruct (NameMap.find v.(varName) st.(registers)) as [x | ] eqn:Eregisters. { exact x. }
+  destruct (NameMap.find v.(varName) st.(variables)) as [x | ] eqn:Evariables. { exact x. }
+  exfalso.
+  rewrite <- NameMapFacts.not_find_in_iff in *.
+  destruct input_wf.
+  - apply Evariables. clear Evariables. clear Eregisters.
+    destruct st as [exts regs vars]. simpl in *.
+    destruct vars as [var_map vars_wf].
+    simpl.
+    rewrite Forall_forall in vars_wf.
+    apply vars_wf in H. clear vars_wf.
+    funelim (variable_in_map var_map v).
+    simp variable_in_map in *.
+  - apply Eregisters. clear Evariables. clear Eregisters.
+    rewrite Exists_exists in H.
+    destruct H as [r [H1 H2]].
+    destruct st as [exts regs vars]. simpl in *.
+    destruct regs as [reg_map regs_wf].
+    simpl in *.
+    rewrite Forall_forall in regs_wf.
+    apply regs_wf in H1.
+    funelim (register_in_map reg_map r).
+    funelim (var_reg_match v (MkRegister reg_type n init driver)).
+    simp register_in_map in *.
+    simp var_reg_match in *.
+    simpl in *.
+    inversion H2; subst.
+    assumption.
+Qed.
+
+Lemma input_run_width : forall {c} (st : CircuitState c) i input_wf,
+    width (input_run st i input_wf) = input_width i.
+Proof.
+Admitted.
+
+Lemma variable_in_map_extend : forall (k : NameMap.key) (var : variable) (x: bv) (m : NameMap.t bv),
+    variable_in_map m var -> variable_in_map (NameMap.add k x m) var.
+Proof.
+  intros.
+  funelim (variable_in_map m var).
+  simp variable_in_map in *.
+  apply NameMapFacts.add_in_iff.
+  auto.
+Qed.
+
+Equations cell_run {c} (st : CircuitState c) (cl : cell) (cell_wf : cell_in_circuit c cl) : CircuitState c :=
+  cell_run st (Add (OutVar (Var _ out)) in1 in2 inputs_match output_match) cell_wf :=
+    let val1 := input_run st in1 _ in
+    let val2 := input_run st in2 _ in
+    let result := bv_add_truncate val1 val2 _ in
     MkCircuitState
       (external st)
       (registers st)
-      (NameMap.add out result (variables st));
+      (MkVariableState (NameMap.add out result (variables st)) _);
   (* TODO: Cells other than Add *)
-  cell_run st _ := st.
-
+  cell_run st _ _ := st.
+Next Obligation.
+  simp cell_in_circuit in cell_wf.
+  decompose [and] cell_wf.
+  assumption.
+Qed.
+Next Obligation.
+  simp cell_in_circuit in cell_wf.
+  decompose [and] cell_wf.
+  assumption.
+Qed.
+Next Obligation.
+  repeat rewrite input_run_width.
+  assumption.
+Qed.
+Next Obligation.
+  destruct st as [exts regs vars].
+  destruct vars as [vars_map vars_wf].
+  simpl in *.
+  pose proof vars_wf as vars_wf_forall.
+  rewrite Forall_forall.
+  rewrite Forall_forall in vars_wf_forall.
+  auto using variable_in_map_extend.
+Qed.
 
 Equations circuit_run
   (fext : ExternalState)
